two ways of writing btrees

btrees/verif_relation_mem.v
@@ -1,12 +1,175 @@
-(** * verif_btrees.v: Correctness proof of relation_mem.c *)
+(** * verif_relation_mem.v: Correctness proof of relation_mem.c *)
 
 Require Import VST.floyd.proofauto.
 Require Import VST.floyd.library.
 Require Import relation_mem.
 Instance CompSpecs : compspecs. make_compspecs prog. Defined.
-Definition Vprog : varspecs.  mk_varspecs prog. Defined.
+Definition Vprog : varspecs. mk_varspecs prog. Defined.
 
 Require Import VST.msl.wand_frame.
 Require Import VST.msl.iter_sepcon.
 Require Import VST.floyd.reassoc_seq.
 Require Import VST.floyd.field_at_wand.
+
+Definition key := Z.            (* unsigned long in C *)
+
+Section BTrees.
+Variable V : Type.
+Variable b : nat.
+
+Inductive entry: Type :=
+     | ptr0: node -> entry
+     | keyval: key -> V -> entry
+     | keychild: key -> node -> entry
+with node: Type :=
+     | nil: node
+     | cons: entry -> node -> node.
+(* every list of keychilds begins with a ptr0 *)
+
+Fixpoint max_nat (m : nat) (n : nat) : nat :=
+  match m with
+  | O => n
+  | S m' => (match n with
+             | O => m
+             | S n' => S (max_nat m' n')
+             end)
+  end.
+
+Fixpoint node_depth (n:node) : nat :=
+  match n with
+  | nil => O
+  | cons e n' => max_nat (entry_depth e) (node_depth n')
+  end
+with entry_depth (e:entry) : nat :=
+  match e with
+  | ptr0 n => S (node_depth n)
+  | keyval _ _ => S O
+  | keychild _ n => S (node_depth n)
+  end.
+
+Fixpoint node_length (n:node) : nat :=
+  match n with
+  | nil => O
+  | cons _ n' => S (node_length n')
+  end.
+
+Definition cursor: Type := list nat. (* ancestors index *)
+
+Fixpoint nth_child (i:nat) (n:node) : option node :=
+  match i with
+  | O => match n with
+         | nil => None
+         | cons e _ => match e with
+                       | ptr0 n' => Some n'
+                       | keyval _ _ => None
+                       | keychild _ n' => Some n'
+                       end
+         end
+  | S i' => match n with
+            | nil => None
+            | cons _ n' => nth_child i' n'
+            end
+  end.
+
+Fixpoint nth_val (i:nat) (n:node) : option V :=
+  match i with
+  | O => match n with
+         | nil => None
+         | cons e _ => match e with
+                       | ptr0 _ => None
+                       | keyval _ v => Some v
+                       | keychild _ _ => None
+                       end
+         end
+  | S i' => match n with
+            | nil => None
+            | cons _ n' => nth_val i' n'
+            end
+  end.
+
+Fixpoint is_valid (c:cursor) (n:node):= (* cursor is reversed *)
+  match c with
+  | [] => match n with
+          | nil => True
+          | _ => False
+          end
+  | i::c' => match c' with
+             | [] => match nth_val i n with
+                     | Some _ => True
+                     | None => False
+                     end
+             | _ => match nth_child i n with
+                    | Some n' => is_valid c' n'
+                    | None => False
+                    end
+             end
+  end.
+
+Definition empty_btree: node := nil.
+Definition empty_cursor: cursor := [].
+
+Inductive partial_cursor_valid : cursor -> node -> node -> Prop :=
+| pcv_emp: forall n, partial_cursor_valid [] n n
+| pcv_root: forall (i:nat) n n', le i (node_length n) ->
+                      nth_child i n = Some n' ->
+                      partial_cursor_valid [i] n' n
+| pcv_cons: forall i c curr curr' n, partial_cursor_valid c curr n ->
+                                     le i (node_length curr) -> 
+                                     nth_child i curr = Some curr' ->
+                                     partial_cursor_valid (i::c) curr' n.
+
+Inductive cursor_valid : cursor -> node -> Prop :=
+| valid_val: forall c curr n i v, partial_cursor_valid c curr n ->
+                                  nth_val i curr = Some v ->
+                                  cursor_valid c n.
+                      
+Inductive get_value : cursor -> node -> V -> Prop :=
+| get: forall c curr n i v, partial_cursor_valid c curr n ->
+                            nth_val i curr = Some v ->
+                            get_value c n v.
+
+
+
+
+Fixpoint node_to_list (n:node) : list entry :=
+  match n with
+  | nil => []
+  | cons e n' =>
+    match e with
+    | ptr0 n'' => node_to_list n'
+    | keyval k v => (keyval k v)::node_to_list n'
+    | keychild k c => (keychild k c)::node_to_list n'
+    end
+  end.
+
+Definition node_to_ptr0 (n:node) : option node :=
+  match n with
+  | nil => None
+  | cons e n' =>
+    match e with
+    | ptr0 n'' => Some n''
+    | _ => None
+    end
+  end.
+
+Definition btnode_rep (n:node) (p:val) : mpred :=
+  EX nvl: list entry, EX ptr0: option node, EX pptr0: val,
+     !!(nvl = node_to_list n) && !!(ptr0 = node_to_ptr0 n) &&
+     (* if ptr0 = Some, then btnode_rep ptr0 pptr0 *)
+     malloc_token Tsh (Tstruct _BtNode noattr) p
+     (* * field_at Tsh (Tstruct _BtNode noattr) [StructField _isLeaf] (if ptr0=None then false else true) p * *)
+     (* field_at Tsh (Tstruct _BtNode noattr) [StructField _numKeys] (Zlength nvl) p * *)
+     (* field_at Tsh (Tstruct _BtNode noattr) [StructField _ptr0] (ptr0) p * (* should be a val *) *)
+     (* field_at Tsh (Tstruct _BtNode noattr) [StructField _entries] (nvl) p (* this isn't right *) *).
+
+Definition value_rep (v:V) (p:val):mpred := emp. (* todo *)
+
+Definition key_rep (k:key) (p:val):mpred := emp. (* todo *)
+
+Definition entry_rep (e:entry) (p:val) : mpred :=
+  match e with
+  | ptr0 _ => emp
+  | keyval k v => value_rep v p * key_rep k p
+  | keychild k c => key_rep k p * btnode_rep c p
+  end.
+                    (* not p but the corresponding field *)
