btrees/bad.v
@@ -1,0 +1,68 @@
+(** * verif_btrees.v: Correctness proof of relation_mem.c *)
+
+Require Import VST.floyd.proofauto.
+Require Import VST.floyd.library.
+Require Import relation_mem.
+Instance CompSpecs : compspecs. make_compspecs prog. Defined.
+Definition Vprog : varspecs.  mk_varspecs prog. Defined.
+
+Require Import VST.msl.wand_frame.
+Require Import VST.msl.iter_sepcon.
+Require Import VST.floyd.reassoc_seq.
+Require Import VST.floyd.field_at_wand.
+
+Definition key := Z.            (* unsigned long in C *)
+
+Section BTrees.
+Variable V : Type.
+Variable b : nat.
+
+Inductive node: Type :=
+| L: leafnode -> node
+| I: internnode -> node
+with leafnode: Type :=
+| LN: leafnode
+| LE: valentrylist -> leafnode
+with internnode: Type :=
+| IN: internnode
+| IE: node -> childentrylist -> internnode (* first node is ptr0 *)
+with valentrylist: Type :=      (* nonempty *)
+| VELO: key -> V -> valentrylist
+| VELC: key -> V -> valentrylist -> valentrylist
+with childentrylist: Type :=    (* nonempty *)
+| CELO: key -> node -> childentrylist
+| CELC: key -> node -> childentrylist -> childentrylist.
+
+Definition cursor: Type := list Z. (* ancestors index *)
+
+Definition empty_tree: node := L LN.
+
+Fixpoint vel_length (vl: valentrylist) :=
+  match vl with
+  | VELO _ _ => 1
+  | VELC _ _ vl' => 1+ vel_length vl'
+  end.
+
+Fixpoint cel_length (cl: childentrylist) :=
+  match cl with
+  | CELO _ _ => 1
+  | CELC _ _ cl' => 1+ cel_length cl'
+  end.
+
+Definition node_length (n:node):=
+  match n with
+  | L l => match l with
+           | LN => 0
+           | LE vl => vel_length vl
+           end
+  | I i => match i with
+           | IN => 0
+           | IE ptr0 cl => cel_length cl
+           end
+  end.
+
+Lemma empty_empty_tree: node_length empty_tree = 0.
+Proof. auto. Qed.
+
+Definition cursor_valid: cursor -> node -> Prop.
+  Admitted.
